src/impl/TLS13.Impl.Driver.Pairing.fsti
@@ -253,7 +253,7 @@ let client_server_driver_supported_profile_derived_state_inputs
   (server:CS.connection_state)
   : prop =
   CS.paired_x25519_key_shares client server /\
-  CS.paired_handshake_events client server
+  CS.paired_key_derivation_checkpoints client server
 
 noextract
 let client_x25519_key_share_projection
@@ -295,7 +295,7 @@ let client_server_driver_handshake_projection_inputs
   (client:CS.connection_state)
   (server:CS.connection_state)
   : prop =
-  CS.paired_handshake_events client server
+  CS.paired_key_derivation_checkpoints client server
 
 noextract
 let client_server_driver_supported_profile_derived_projection_inputs
@@ -313,13 +313,13 @@ val lemma_client_server_driver_paired_x25519_key_shares_from_projection_inputs
         client_server_driver_x25519_projection_inputs client server)
       (ensures CS.paired_x25519_key_shares client server)
 
-val lemma_client_server_driver_paired_handshake_events_from_projection_inputs
+val lemma_client_server_driver_paired_key_derivation_checkpoints_from_projection_inputs
   (client:CS.connection_state)
   (server:CS.connection_state)
   : Lemma
       (requires
         client_server_driver_handshake_projection_inputs client server)
-      (ensures CS.paired_handshake_events client server)
+      (ensures CS.paired_key_derivation_checkpoints client server)
 
 val lemma_client_server_driver_supported_profile_derived_state_inputs_from_projection_inputs
   (client:CS.connection_state)
