src/spec/TLS13.ConnectionState.Lemmas.fsti
@@ -214,7 +214,7 @@ val lemma_paired_supported_profile_all_derived_key_material_agrees
         paired_x25519_key_shares client server /\
         connection_supported_profile_key_schedule_lineage client /\
         connection_supported_profile_key_schedule_lineage server /\
-        paired_handshake_events client server)
+        paired_key_derivation_checkpoints client server)
       (ensures
         supported_profile_all_derived_key_material_agrees client server)
 
